src/Helpers/List.v
@@ -717,3 +717,74 @@ Proof.
   f_equiv.
   rewrite Permutation_swap //.
 Qed.
+
+Lemma subslice_app_length {A} n m (l0 l1 : list A) :
+  subslice ((length l0) + n) ((length l0) + m) (l0 ++ l1) =
+  subslice n m l1.
+Proof. by rewrite /subslice take_app_add drop_app_add. Qed.
+
+Lemma join_lookup_Some_same_length'' {A} i c (x : list A) ls :
+  Forall (λ x, length x = c) ls →
+  ls !! i = Some x →
+  x = subslice (i * c) (S i * c) (mjoin ls).
+Proof.
+  revert i. induction ls.
+  { intros ?? Hlook. by rewrite lookup_nil in Hlook. }
+  intros ? Hc ?.
+  apply Forall_cons in Hc as [<- ?].
+  destruct i.
+  - rewrite subslice_from_start.
+    rewrite take_app_length'; [|lia].
+    naive_solver.
+  - rewrite subslice_app_length.
+    by apply IHls.
+Qed.
+
+Lemma subslice_singleton {A} l n (x : A) :
+  l !! n = Some x →
+  subslice n (S n) l = [x].
+Proof.
+  intros Hlook. rewrite /subslice.
+  eapply lookup_lt_Some in Hlook as ?.
+  eapply take_drop_middle in Hlook as <-.
+  rewrite cons_middle.
+  rewrite (assoc app).
+  rewrite take_app_length'.
+  2: { rewrite app_length length_take. simpl. lia. }
+  rewrite drop_app_length'; [done|].
+  rewrite length_take. lia.
+Qed.
+
+Local Lemma join_subslice_aux {A} i k c (ls : list $ list A) :
+  i ≤ i + k ≤ length ls →
+  Forall (λ x, length x = c) ls →
+  mjoin (subslice i (k + i) ls) = subslice (i * c) ((k + i) * c) (mjoin ls).
+Proof.
+  intros. induction k.
+  { by rewrite !subslice_zero_length. }
+  rewrite (subslice_split_r _ (k + i)); [|lia..].
+  rewrite join_app.
+  rewrite (subslice_split_r (i * c) ((k + i) * c)); [|lia|].
+  2: {
+    rewrite length_join.
+    rewrite (sum_list_fmap_same c); [|done].
+    eapply Nat.mul_le_mono_r. lia. }
+  f_equal. { apply IHk. lia. }
+  clear IHk.
+  destruct (list_lookup_lt ls (k + i)) as [x Hlook]; [lia|].
+  pose proof Hlook as Hlook0.
+  replace (S k + i) with (S (k + i)) by lia.
+  eapply subslice_singleton in Hlook0 as ->.
+  list_simplifier.
+  by rewrite -(join_lookup_Some_same_length'' _ _ x).
+Qed.
+
+Lemma join_subslice {A} i j c (ls : list $ list A) :
+  i ≤ j ≤ length ls →
+  Forall (λ x, length x = c) ls →
+  mjoin (subslice i j ls) = subslice (i * c) (j * c) (mjoin ls).
+Proof.
+  intros.
+  replace (j) with ((j - i) + i) by lia.
+  eapply join_subslice_aux; [lia|done].
+Qed.
